Locally_Nameless_Lambda_Calculus/LN_Lambda_Term.thy
@@ -50,6 +50,65 @@ inductive locally_closed :: "('\<tau>, '\<Sigma>, '\<V>) preterm \<Rightarrow> b
   Abs: "locally_closed (Abs \<tau> t)"
     if "\<And>x. x |\<notin>| \<X> \<Longrightarrow> locally_closed (subst_bound 0 (Free x) t)"
 
+definition body where
+  "body t \<longleftrightarrow> (\<exists>\<X>. \<forall>x. x |\<notin>| \<X> \<longrightarrow> locally_closed (subst_bound 0 (Free x) t))"
+
+text \<open>A structural, level-indexed notion of local closure: \<open>locally_closed_at k t\<close> holds when every
+  dangling bound index of \<open>t\<close> is smaller than \<open>k\<close>. \<^bold>\<open>Note:\<close> constant parameters are required to be
+  closed (level \<open>0\<close>), matching the fact that \<^const>\<open>subst_bound\<close> and \<open>subst_free\<close> treat them
+  opaquely (they never descend into them); with the naive rule \<open>list_all (locally_closed_at k) ts\<close>
+  the equivalence with \<^const>\<open>locally_closed\<close> below would fail.\<close>
+
+inductive locally_closed_at :: "nat \<Rightarrow> ('\<tau>, '\<Sigma>, '\<V>) preterm \<Rightarrow> bool" where
+  Bound: "locally_closed_at k (Bound i)" if "i < k" |
+  Const: "locally_closed_at k (Const c \<tau>s ts)" if "list_all (locally_closed_at 0) ts" for k c \<tau>s ts |
+  Free: "locally_closed_at k (Free f)" |
+  App: "locally_closed_at k (App t\<^sub>1 t\<^sub>2)" if "locally_closed_at k t\<^sub>1" and "locally_closed_at k t\<^sub>2" |
+  Abs: "locally_closed_at k (Abs \<tau> t)" if "locally_closed_at (Suc k) t"
+
+lemma locally_closed_at_Bound_iff[simp]: "locally_closed_at k (Bound i) \<longleftrightarrow> i < k"
+  by (auto elim: locally_closed_at.cases intro: locally_closed_at.Bound)
+
+lemma locally_closed_at_Free[simp]: "locally_closed_at k (Free f)"
+  by (rule locally_closed_at.Free)
+
+lemma locally_closed_App_iff: "locally_closed (App t\<^sub>1 t\<^sub>2) \<longleftrightarrow> locally_closed t\<^sub>1 \<and> locally_closed t\<^sub>2"
+  by (auto elim: locally_closed.cases intro: locally_closed.App)
+
+lemma locally_closed_at_App_iff[simp]:
+  "locally_closed_at k (App t\<^sub>1 t\<^sub>2) \<longleftrightarrow> locally_closed_at k t\<^sub>1 \<and> locally_closed_at k t\<^sub>2"
+  by (auto elim: locally_closed_at.cases intro: locally_closed_at.App)
+
+lemma locally_closed_Const_iff[simp]:
+  "locally_closed (Const \<kappa> \<tau>s ts) \<longleftrightarrow> (\<forall>t \<in> set ts. locally_closed t)"
+  by (metis list.pred_set locally_closed.simps preterm.distinct(1,5) preterm.inject(1)
+      preterm.simps(13))
+
+lemma locall_closed_Abs_iff_body: "locally_closed (Abs \<tau> t) \<longleftrightarrow> body t"
+  unfolding locally_closed.simps[of "Abs _ _", simplified] body_def ..
+
+lemma body_App_iff: "body (App t\<^sub>1 t\<^sub>2) \<longleftrightarrow> body t\<^sub>1 \<and> body t\<^sub>2"
+  unfolding body_def by (auto simp add: locally_closed_App_iff)
+
+lemma locally_closed_at_Abs_iff[simp]:
+  "locally_closed_at k (Abs \<tau> t) \<longleftrightarrow> locally_closed_at (Suc k) t"
+  by (auto elim: locally_closed_at.cases intro: locally_closed_at.Abs)
+
+lemma locally_closed_at_Const_iff[simp]:
+  "locally_closed_at k (Const c \<tau>s ts) \<longleftrightarrow> (\<forall>t \<in> set ts. locally_closed_at 0 t)"
+  by (auto elim: locally_closed_at.cases intro: locally_closed_at.Const simp: list.pred_set)
+
+text \<open>Opening a fresh variable lowers the level by one, and vice versa (local closure ignores free
+  variables, so no freshness side condition is needed).\<close>
+
+lemma locally_closed_at_subst_bound_Free:
+  "locally_closed_at (Suc k) t \<Longrightarrow> locally_closed_at k (subst_bound k (Free x) t)"
+  by (induction t arbitrary: k) auto
+
+lemma locally_closed_at_Suc_if_subst_bound_Free:
+  "locally_closed_at k (subst_bound k (Free x) t) \<Longrightarrow> locally_closed_at (Suc k) t"
+  by (induction t arbitrary: k) (auto split: if_splits)
+
 primrec subst_free
   :: "'\<V> \<Rightarrow> ('\<tau>, '\<Sigma>, '\<V>) preterm \<Rightarrow> ('\<tau>, '\<Sigma>, '\<V>) preterm \<Rightarrow> ('\<tau>, '\<Sigma>, '\<V>) preterm" where
   "subst_free x u (Const c \<tau>s ts) = Const c \<tau>s ts"|
@@ -58,14 +117,82 @@ primrec subst_free
   "subst_free x u (App t\<^sub>1 t\<^sub>2) = App (subst_free x u t\<^sub>1) (subst_free x u t\<^sub>2)" |
   "subst_free x u (Abs \<tau> t) = Abs \<tau> (subst_free x u t)"
 
-definition body where
-  "body t \<longleftrightarrow> (\<exists>\<X>. \<forall>x. x |\<notin>| \<X> \<longrightarrow> locally_closed (subst_bound 0 (Free x) t))"
+lemma size_subst_bound_Free[simp]: "size (subst_bound n (Free x) t) = size t"
+  by (induction t arbitrary: n) simp_all
 
-lemma locally_closed_App_iff: "locally_closed (App t\<^sub>1 t\<^sub>2) \<longleftrightarrow> locally_closed t\<^sub>1 \<and> locally_closed t\<^sub>2"
-  by (auto elim: locally_closed.cases intro: locally_closed.App)
+text \<open>Over an infinite variable type, \<^const>\<open>locally_closed\<close> and \<^const>\<open>body\<close> coincide with
+  \<^const>\<open>locally_closed_at\<close> at levels \<open>0\<close> and \<open>1\<close>. (Infinitely many variables are needed to rule out the
+  spurious models of the cofinite \<^const>\<open>locally_closed\<close> over finite variable types.)\<close>
 
-lemma locall_closed_Abs_iff_body: "locally_closed (Abs \<tau> t) \<longleftrightarrow> body t"
-  unfolding locally_closed.simps[of "Abs _ _", simplified] body_def ..
+lemma locally_closed_iff_locally_closed_at:
+  fixes t :: "('\<tau>, '\<Sigma>, '\<V>) preterm"
+  assumes inf_vars: "infinite (UNIV :: '\<V> set)"
+  shows "locally_closed t \<longleftrightarrow> locally_closed_at 0 t"
+proof (induction t rule: measure_induct_rule[where f = size])
+  case (less t)
+  show ?case
+  proof (cases t)
+    case (Const c \<tau>s ts)
+    have "size t' < size t" if "t' \<in> set ts" for t'
+    proof -
+      have "size t' \<le> size_list size ts"
+        by (rule size_list_estimation'[OF that order_refl])
+      then show ?thesis by (simp add: Const)
+    qed
+    then show ?thesis
+      using less.IH by (auto simp: Const)
+  next
+    case (Free x)
+    then show ?thesis by (simp add: locally_closed.Free)
+  next
+    case (Bound i)
+    then show ?thesis by (simp add: locally_closed.simps[of "Bound _"])
+  next
+    case (App t\<^sub>1 t\<^sub>2)
+    then show ?thesis
+      using less.IH by (auto simp: locally_closed_App_iff)
+  next
+    case (Abs \<tau> s)
+    have "body s \<longleftrightarrow> locally_closed_at (Suc 0) s"
+    proof
+      assume "body s"
+      then obtain \<X> :: "'\<V> fset" where
+        X: "\<And>x. x |\<notin>| \<X> \<Longrightarrow> locally_closed (subst_bound 0 (Free x) s)"
+        unfolding body_def by blast
+      obtain x :: '\<V> where "x |\<notin>| \<X>"
+        using inf_vars by (metis ex_new_if_finite finite_fset)
+      from X[OF this] have "locally_closed (subst_bound 0 (Free x) s)" .
+      moreover have "size (subst_bound 0 (Free x) s) < size t"
+        by (simp add: Abs)
+      ultimately have "locally_closed_at 0 (subst_bound 0 (Free x) s)"
+        using less.IH by blast
+      then show "locally_closed_at (Suc 0) s"
+        by (rule locally_closed_at_Suc_if_subst_bound_Free)
+    next
+      assume "locally_closed_at (Suc 0) s"
+      have "locally_closed (subst_bound 0 (Free x) s)" for x
+      proof -
+        have "locally_closed_at 0 (subst_bound 0 (Free x) s)"
+          using locally_closed_at_subst_bound_Free[OF \<open>locally_closed_at (Suc 0) s\<close>] by simp
+        moreover have "size (subst_bound 0 (Free x) s) < size t"
+          by (simp add: Abs)
+        ultimately show ?thesis
+          using less.IH by blast
+      qed
+      then show "body s"
+        unfolding body_def by blast
+    qed
+    then show ?thesis
+      by (simp add: Abs locall_closed_Abs_iff_body)
+  qed
+qed
+
+lemma body_iff_locally_closed_at:
+  fixes t :: "('\<tau>, '\<Sigma>, '\<V>) preterm"
+  assumes inf_vars: "infinite (UNIV :: '\<V> set)"
+  shows "body t \<longleftrightarrow> locally_closed_at (Suc 0) t"
+  by (metis locally_closed_iff_locally_closed_at[OF inf_vars] locally_closed_at_Abs_iff
+      locall_closed_Abs_iff_body)
 
 lemma subst_bound_subst_bound_Free_idem[simp]:
   "subst_bound n u (subst_bound n (Free x) t) = subst_bound n (Free x) t"
@@ -118,37 +245,26 @@ next
     by (metis IH' nat.distinct(1) subst_bound.simps(5) subst_bound_subst_bound_Free_idem)
 qed
 
-lemma subst_free_term_subst_bound_Free_eq_subst_bound_term:
+
+text \<open>Chargu\<eacute>raud's \<open>subst_open\<close>: substitution commutes with opening. His proof generalises to an
+  arbitrary index and, in the \<^const>\<open>Free\<close> case, uses \<open>open_rec_lc\<close> (here
+  \<open>subst_bound_ident_if_locally_closed\<close>) to see that opening does not affect the locally closed term
+  \<open>u\<close>. That auxiliary needs \<open>infinite (UNIV :: '\<V> set)\<close> in this development (the \<open>Abs\<close> rule of
+  \<^const>\<open>locally_closed\<close> is cofinite), which corresponds to Chargu\<eacute>raud's atoms being infinite; over a
+  finite variable type \<^const>\<open>locally_closed\<close> can hold spuriously and the statement is refutable.\<close>
+
+lemma subst_open:
+  fixes t :: "('\<tau>, '\<Sigma>, '\<V>) preterm"
+  assumes inf_vars: "infinite (UNIV :: '\<V> set)"
+  assumes "locally_closed u"
+  shows "subst_free x u (subst_bound k v t) = subst_bound k (subst_free x u v) (subst_free x u t)"
+  by (induction t arbitrary: k)
+    (simp_all add: subst_bound_ident_if_locally_closed[OF inf_vars \<open>locally_closed u\<close>])
+
+lemma subst_free_subst_bound_Free_eq_subst_bound:
   assumes "x \<notin> free_vars t"
   shows "subst_free x u (subst_bound n (Free x) t) = subst_bound n u t"
-  using assms
-proof (induction t arbitrary: n rule: preterm.induct)
-  case (Const c \<tau>s ts)
-  then show ?case
-    by simp
-next
-  case (Free y)
-  then have "x \<noteq> y"
-    by simp
-  then show ?case
-    by simp
-next
-  case (Bound i)
-  then show ?case
-    by (auto split: if_split)
-next
-  case (App t1 t2)
-  then show ?case
-    by simp
-next
-  case (Abs \<tau> t)
-  have "x \<notin> free_vars t"
-    using Abs.prems by simp
-  then have "\<And>n. subst_free x u (subst_bound n (Free x) t) = subst_bound n u t"
-    using Abs.IH by simp
-  then show ?case
-    by simp
-qed
+  using assms by (induction t arbitrary: n) auto
 
 lemma subst_free_commutes_with_subst_bound_Free:
   fixes t :: "('\<tau>, '\<Sigma>, '\<V>) preterm"
@@ -243,14 +359,27 @@ lemma body_Abs_if_body:
   fixes t :: "('\<tau>, '\<Sigma>, '\<V>) preterm"
   assumes inf_vars: "infinite (UNIV :: '\<V> set)"
   shows "body t \<Longrightarrow> body (Abs \<tau> t)"
-  unfolding body_def
-  apply (induction t)
-      apply (simp_all add: locally_closed.intros)
-    apply (metis Abs subst_bound.simps(3))
-  using subst_bound_ident_if_locally_closed[OF inf_vars]
-   apply (metis Abs subst_bound.simps(4,5))
-  using subst_bound_ident_if_locally_closed[OF inf_vars]
-  by (metis Abs subst_bound.simps(5))
+proof (induction t)
+  case (Const x1 x2a x3a)
+  then show ?case
+    by (simp add: body_def locall_closed_Abs_iff_body)
+next
+  case (Free x)
+  then show ?case
+    by (simp add: body_iff_locally_closed_at inf_vars)
+next
+  case (Bound x)
+  then show ?case
+    by (simp add: body_iff_locally_closed_at inf_vars)
+next
+  case (App t1 t2)
+  then show ?case
+    by (simp add: body_iff_locally_closed_at inf_vars)
+next
+  case (Abs x1 t)
+  then show ?case
+    by (metis body_def locall_closed_Abs_iff_body subst_bound_ident_if_locally_closed[OF inf_vars])
+qed
 
 lemma locally_closed_subst_bound:
   fixes t u :: "('\<tau>, '\<Sigma>, '\<V>) preterm"
@@ -267,7 +396,7 @@ proof -
     by (metis Un_iff ex_new_if_finite finite_Un finite_fset finite_vars_term inf_vars)
 
   then obtain "subst_free x u (subst_bound 0 (Free x) t) = subst_bound 0 u t"
-    using subst_free_term_subst_bound_Free_eq_subst_bound_term by metis
+    using subst_free_subst_bound_Free_eq_subst_bound by metis
 
   moreover have "locally_closed (subst_free x u (subst_bound 0 (Free x) t))"
   proof (rule locally_closed_subst_free[OF inf_vars])
